# See details within this document for linkage to specification and purpose.
# This ontology file is a non-normative supporting document.

# Comments/Questions
# What's with the owl:Individual (it's not in the non-normative owl ttl, owl individual axiom is described as class instance here https://www.ida.liu.se/research/semanticweb/events/SemWebCourse2018/OWL_basics.pdf)
# What's the current status of the terms with status testing?
# Should the Term statuses actually be URIs? (they're not described as such in sw-vocab but hey, need to understand the rationale)

## Ontology preferred namespace prefix and URI
@prefix ldp: <http://www.w3.org/ns/ldp#> .

## Other namespaces used
@prefix dcterms: <http://purl.org/dc/terms/> .
@prefix foaf: <http://xmlns.com/foaf/0.1/> .
@prefix owl: <http://www.w3.org/2002/07/owl#> .
@prefix rdf: <http://www.w3.org/1999/02/22-rdf-syntax-ns#> .
@prefix rdfs: <http://www.w3.org/2000/01/rdf-schema#> .
@prefix vann: <http://purl.org/vocab/vann/> .
@prefix vs: <http://www.w3.org/2003/06/sw-vocab-status/ns#> .
@prefix xsd: <http://www.w3.org/2001/XMLSchema#> .

## Ontology
<http://www.w3.org/ns/ldp#>
    a owl:Ontology ;
    rdfs:label "W3C Linked Data Platform (LDP)" ;
    rdfs:comment "This ontology provides an informal representation of the concepts and terms as defined in the LDP specification. Consult the LDP specification for normative reference." ;
    dcterms:description "Vocabulary URIs defined in the Linked Data Platform (LDP) namespace." ;
    dcterms:title "The W3C Linked Data Platform (LDP) Vocabulary" ;
    dcterms:publisher <http://www.w3.org/data#W3C> ;
    dcterms:creator
        [ foaf:name "Ashok Malhotra" ],
        [ foaf:name "John Arwe" ],
        [ foaf:name "Steve Speicher" ] ;
    foaf:maker
        [ foaf:homepage <http://www.w3.org/2012/ldp> ] ;
    dcterms:created "2015-02-26"^^xsd:date ;
    vann:preferredNamespaceUri "http://www.w3.org/ns/ldp#" ;
    vann:preferredNamespacePrefix "ldp" ;
    rdfs:seeAlso
        <http://www.w3.org/2012/ldp>,
        <http://www.w3.org/TR/ldp-ucr/>,
        <http://www.w3.org/TR/ldp/>,
        <http://www.w3.org/TR/ldp-paging/>,
        <http://www.w3.org/2011/09/LinkedData/> .

## Class
ldp:Resource
    a rdfs:Class;
    rdfs:label "Resource" ;
    rdfs:comment "A HTTP-addressable resource whose lifecycle is managed by a LDP server." ;
    rdfs:isDefinedBy <http://www.w3.org/ns/ldp#> ;
    vs:term_status "stable" .

ldp:RDFSource
    a rdfs:Class ;
    rdfs:label "RDFSource" .
    rdfs:comment "A Linked Data Platform Resource (LDPR) whose state is represented as RDF." ;
    rdfs:isDefinedBy <http://www.w3.org/ns/ldp#> ;
    rdfs:subClassOf ldp:Resource ;
    vs:term_status "stable" .

ldp:NonRDFSource
    a rdfs:Class;
    rdfs:label "NonRDFSource" ;
    rdfs:comment "A Linked Data Platform Resource (LDPR) whose state is NOT represented as RDF." ;
    rdfs:isDefinedBy <http://www.w3.org/ns/ldp#> ;
    rdfs:subClassOf ldp:Resource ;
    vs:term_status "stable" .

ldp:Container
    a rdfs:Class ;
    rdfs:label "Container" ;
    rdfs:comment "A Linked Data Platform RDF Source (LDP-RS) that also conforms to additional patterns and conventions for managing membership. Readers should refer to the specification defining this ontology for the list of behaviors associated with it." ;
    rdfs:isDefinedBy <http://www.w3.org/ns/ldp#> ;
    rdfs:subClassOf ldp:RDFSource ;
    vs:term_status "stable" .

ldp:BasicContainer
    a rdfs:Class;
    rdfs:label "BasicContainer" ;
    rdfs:comment "An LDPC that uses a predefined predicate to simply link to its contained resources." ;
    rdfs:isDefinedBy <http://www.w3.org/ns/ldp#> ;
    rdfs:subClassOf ldp:Container ;
    vs:term_status "stable" .

ldp:DirectContainer
    a rdfs:Class ;
    rdfs:label "DirectContainer" ;
    rdfs:comment "An LDPC that is similar to a LDP-DC but it allows an indirection with the ability to list as member a resource, such as a URI representing a real-world object, that is different from the resource that is created." ;
    rdfs:isDefinedBy <http://www.w3.org/ns/ldp#> ;
    rdfs:subClassOf ldp:Container ;
    vs:term_status "stable" .

ldp:IndirectContainer
    a rdfs:Class ;
    rdfs:label "IndirectContainer" ;
    rdfs:comment "An LDPC that has the flexibility of choosing what form the membership triples take." ;
    rdfs:isDefinedBy <http://www.w3.org/ns/ldp#> ;
    rdfs:subClassOf ldp:Container ;
    vs:term_status "stable" .

ldp:Page
    a rdfs:Class ;
    rdfs:label "Page" ;
    rdfs:comment "URI signifying that the resource is an in-sequence page resource, as defined by LDP Paging. Typically used on Link rel='type' response headers." ;
    rdfs:isDefinedBy <http://www.w3.org/ns/ldp#> ;
    vs:term_status "testing" .

ldp:PageSortCriterion
    a rdfs:Class ;
    rdfs:label "PageSortCriterion" ;
    rdfs:comment "Element in the list of sorting criteria used by the server to assign container members to pages." ;
    rdfs:isDefinedBy <http://www.w3.org/ns/ldp#> ;
    vs:term_status "testing" .

## Individual
ldp:MemberSubject
    a owl:Individual;
    rdfs:comment "Used to indicate default and typical behavior for ldp:insertedContentRelation, where the member-URI value in the membership triple added when a creation request is successful is the URI assigned to the newly created resource.";
    vs:term_status "stable";
    rdfs:isDefinedBy ldp:;
    rdfs:label "MemberSubject".

ldp:PreferContainment
    a owl:Individual;
    rdfs:comment "URI identifying a LDPC's containment triples, for example to allow clients to express interest in receiving them.";
    vs:term_status "stable";
    rdfs:isDefinedBy ldp:;
    rdfs:label "PreferContainment".

ldp:PreferMembership
    a owl:Individual;
    rdfs:comment "URI identifying a LDPC's membership triples, for example to allow clients to express interest in receiving them.";
    vs:term_status "stable";
    rdfs:isDefinedBy ldp:;
    rdfs:label "PreferMembership".

ldp:PreferEmptyContainer
    a owl:Individual;
    rdfs:comment "Archaic alias for ldp:PreferMinimalContainer";
    vs:term_status "archaic";
    rdfs:isDefinedBy ldp:;
    owl:equivalentProperty ldp:PreferMinimalContainer;
    rdfs:seeAlso ldp:PreferMinimalContainer;
    rdfs:label "PreferEmptyContainer".

ldp:PreferMinimalContainer
    a owl:Individual;
    rdfs:comment "URI identifying the subset of a LDPC's triples present in an empty LDPC, for example to allow clients to express interest in receiving them.  Currently this excludes containment and membership triples, but in the future other exclusions might be added.  This definition is written to automatically exclude those new classes of triples.";
    vs:term_status "stable";
    rdfs:isDefinedBy ldp:;
    rdfs:label "PreferMinimalContainer".

ldp:Ascending
    a owl:Individual;
    rdfs:comment "Ascending order.";
    vs:term_status "testing";
    rdfs:isDefinedBy ldp:;
    rdfs:label "Ascending".

ldp:Descending
    a owl:Individual;
    rdfs:comment "Descending order.";
    vs:term_status "testing";
    rdfs:isDefinedBy ldp:;
    rdfs:label "Descending".

## Property
ldp:hasMemberRelation
    a rdf:Property;
    rdfs:comment "Indicates which predicate is used in membership triples, and that the membership triple pattern is < membership-constant-URI , object-of-hasMemberRelation, member-URI >.";
    vs:term_status "stable";
    rdfs:domain ldp:Container;
    rdfs:isDefinedBy ldp:;
    rdfs:label "hasMemberRelation";
    rdfs:range rdf:Property.

ldp:isMemberOfRelation
    a rdf:Property;
    rdfs:comment "Indicates which predicate is used in membership triples, and that the membership triple pattern is < member-URI , object-of-isMemberOfRelation, membership-constant-URI >.";
    vs:term_status "stable";
    rdfs:domain ldp:Container;
    rdfs:isDefinedBy ldp:;
    rdfs:label "isMemmberOfRelation";
    rdfs:range rdf:Property.

ldp:membershipResource
    a rdf:Property;
    rdfs:comment "Indicates the membership-constant-URI in a membership triple.  Depending upon the membership triple pattern a container uses, as indicated by the presence of ldp:hasMemberRelation or ldp:isMemberOfRelation, the membership-constant-URI might occupy either the subject or object position in membership triples.";
    vs:term_status "stable";
    rdfs:domain ldp:Container;
    rdfs:isDefinedBy ldp:;
    rdfs:label "membershipResource";
    rdfs:range rdfs:Resource.

ldp:insertedContentRelation
    a rdf:Property;
    rdfs:comment "Indicates which triple in a creation request should be used as the member-URI value in the membership triple added when the creation request is successful.";
    vs:term_status "stable";
    rdfs:domain ldp:Container;
    rdfs:isDefinedBy ldp:;
    rdfs:label "insertedContentRelation";
    rdfs:range rdf:Property.

ldp:member
    a rdf:Property;
    rdfs:comment "LDP servers should use this predicate as the membership predicate if there is no obvious predicate from an application vocabulary to use.";
    vs:term_status "stable";
    rdfs:domain ldp:Resource;
    rdfs:isDefinedBy ldp:;
    rdfs:label "member";
    rdfs:range rdfs:Resource.

ldp:contains
    a rdf:Property;
    rdfs:comment "Links a container with resources created through the container.";
    vs:term_status "stable";
    rdfs:domain ldp:Container;
    rdfs:isDefinedBy ldp:;
    rdfs:label "contains";
    rdfs:range rdfs:Resource.

ldp:constrainedBy
    a rdf:Property;
    rdfs:comment "Links a resource with constraints that the server requires requests like creation and update to conform to.";
    vs:term_status "stable";
    rdfs:domain ldp:Resource;
    rdfs:isDefinedBy ldp:;
    rdfs:label "constrainedBy";
    rdfs:range rdfs:Resource.

ldp:pageSortCriteria
    a rdf:Property;
    rdfs:comment "Link to the list of sorting criteria used by the server in a representation.  Typically used on Link response headers as an extension link relation URI in the rel= parameter.";
    vs:term_status "testing";
    rdfs:domain ldp:Page;
    rdfs:isDefinedBy ldp:;
    rdfs:label "pageSortCriteria";
    rdfs:range rdf:List.

ldp:pageSortPredicate
    a rdf:Property;
    rdfs:comment "Predicate used to specify the order of the members across a page sequence's in-sequence page resources; it asserts nothing about the order of members in the representation of a single page.";
    vs:term_status "testing";
    rdfs:domain ldp:PageSortCriterion;
    rdfs:isDefinedBy ldp:;
    rdfs:label "pageSortPredicate";
    rdfs:range rdf:Property.

ldp:pageSortOrder
    a rdf:Property;
    rdfs:comment "The ascending/descending/etc order used to order the members across pages in a page sequence.";
    vs:term_status "testing";
    rdfs:domain ldp:PageSortCriterion;
    rdfs:isDefinedBy ldp:;
    rdfs:label "pageSortOrder";
    rdfs:range rdf:Resource.

ldp:pageSortCollation
    a rdf:Property;
    rdfs:comment "The collation used to order the members across pages in a page sequence when comparing strings.";
    vs:term_status "testing";
    rdfs:domain ldp:PageSortCriterion;
    rdfs:isDefinedBy ldp:;
    rdfs:label "pageSortCollation";
    rdfs:range rdf:Property.

ldp:pageSequence
    a rdf:Property;
    rdfs:comment "Link to a page sequence resource, as defined by LDP Paging.  Typically used to communicate the sorting criteria used to allocate LDPC members to pages.";
    vs:term_status "testing";
    rdfs:isDefinedBy ldp:;
    rdfs:label "Page".

ldp:inbox
    a rdf:Property;
    rdfs:comment "Links a resource to a container where notifications for the resource can be created and discovered.";
    vs:term_status "stable";
    rdfs:isDefinedBy <https://www.w3.org/TR/ldn/>;
    rdfs:label "inbox";
    dcterms:issued "2016-09-29"^^xsd:date;
    dcterms:creator <http://csarven.ca/#i>, <https://rhiaro.co.uk/#me>.
