# See details within this document for linkage to specification and purpose.
# This ontology file is a non-normative supporting document.

# Shape tree ontology

## Ontology preferred namespace prefix and URI
prefix shapetree: <http://www.w3.org/ns/shapetree#>

## Other namespaces used
### Core W3C ontologies (OWL 2 reserved vocabulary)
prefix rdf: <http://www.w3.org/1999/02/22-rdf-syntax-ns#>
prefix rdfs: <http://www.w3.org/2000/01/rdf-schema#>
prefix owl: <http://www.w3.org/2002/07/owl#>
prefix xsd: <http://www.w3.org/2001/XMLSchema#>
### Other ontologies
prefix dcterms: <http://purl.org/dc/terms/>
prefix vann: <http://purl.org/vocab/vann/>

## Ontology
<http://www.w3.org/ns/shapetree>
    a owl:Ontology ;
    rdfs:label "Shape tree ontology"@en ;
    rdfs:isDefinedBy <http://www.w3.org/ns/shapetree> ;
    rdfs:seeAlso
        <https://shapetrees.github.io/specification/primer> ;
    dcterms:issued "2020-07-01"^^xsd:date ;
    dcterms:modified "2020-07-06"^^xsd:date ;
    vann:preferredNamespacePrefix "shapetree" ;
    vann:preferredNamespaceUri "http://www.w3.org/ns/shapetree#"^^xsd:anyURI .


# ShapeTree Class
#############################################################################
# Defines a tree of related resources which combine to enable some task
# see: https://shapetrees.github.io/specification/primer
#############################################################################
shapetree:ShapeTree
  a rdfs:Class ;
  rdfs:comment "Defines a composite data structure including a tree of resources and validation criteria"@en ;
  rdfs:isDefinedBy <http://www.w3.org/ns/shapetree> ;
  rdfs:label "Shape Tree"@en .

#
# Properties in domain of ShapeTree
#
shapetree:expectsType
  a owl:ObjectProperty ;
  rdfs:domain :ShapeTree ;
  rdfs:range [ owl:oneOf ( :ShapeTreeContainer :ShapeTreeResource ) ] ;
  rdfs:comment "Describes the expected type of resource the ShapeTree will validate against."@en ;
  rdfs:isDefinedBy <http://www.w3.org/ns/shapetree> ;
  rdfs:label "Expects Type"@en .

shapetree:contains
  a owl:ObjectProperty ;
  rdfs:domain :ShapeTree ;
  rdfs:range :ShapeTree  ;
  rdfs:comment "Links a ShapeTree to another ShapeTree that is directly contained within its planted ShapeTreeContainer"@en ;
  rdfs:isDefinedBy <http://www.w3.org/ns/shapetree> ;
  rdfs:label "Contains"@en .

shapetree:references
  a owl:ObjectProperty ;
  rdfs:domain :ShapeTree ;
  rdfs:range :ShapeTreeReference ;
  rdfs:isDefinedBy <http://www.w3.org/ns/shapetree> ;
  rdfs:comment "Links a ShapeTree to a ShapeTreeReference"@en ;
  rdfs:label "References"@en .

shapetree:matchesUriTemplate
  a owl:DatatypeProperty ;
  rdfs:domain :ShapeTree ;
  rdfs:range xsd:string ;
  rdfs:comment "Describes a URI Template (RFC 6570) that governs the naming of resources of this Shape Tree"@en ;
  rdfs:isDefinedBy <http://www.w3.org/ns/shapetree> ;
  rdfs:label "Matches URI Template"@en .

shapetree:validatedBy
  a owl:ObjectProperty ;
  rdfs:domain :ShapeTree ;
  rdfs:comment "Links a ShapeTree to a Shape"@en ;
  rdfs:isDefinedBy <http://www.w3.org/ns/shapetree> ;
  rdfs:label "Validated By"@en .

shapetree:supports
  a owl:ObjectProperty ;
  rdfs:domain :ShapeTree ;
  rdfs:range :ShapeTree ;
  rdfs:comment "Describes a relationship wherein a ShapeTree acts as a support for another, for purposes of indexing, aggregation, etc." ;
  rdfs:isDefinedBy <http://www.w3.org/ns/shapetree> ;
  rdfs:label "Supports"@en .

#
# Specific IRIs used by :contains predicate to define behavior
# when a matching ShapeTree with a URI Template is not found.
# These values can be combined, for example,
# :contains :AllowResources :AllowContainers :AllowNonRDFSources is equivalent to :AllowAll
# Example -- <#containerShapeTree> st:contains <#childShapeTree>, st:AllowResources
#
shapetree:AllowResources
  a :ShapeTree ;
  rdfs:comment "If no matching :contains ShapeTree is found, allow if the requested content is a :ShapeTreeResource"@en ;
  rdfs:isDefinedBy <http://www.w3.org/ns/shapetree> ;
  rdfs:label "Allow Resources"@en .

shapetree:AllowContainers
  a :ShapeTree ;
  rdfs:comment "If no matching :contains ShapeTree is found, allow if the requested content is a :ShapeTreeContainer"@en ;
  rdfs:isDefinedBy <http://www.w3.org/ns/shapetree> ;
  rdfs:label "Allow Containers"@en .

shapetree:AllowNonRDFSources
  a :ShapeTree ;
  rdfs:comment "If no matching :contains ShapeTree is found, only allow if the requested content is a :ShapeTreeNonRDFResource"@en ;
  rdfs:isDefinedBy <http://www.w3.org/ns/shapetree> ;
  rdfs:label "Allow NonRDFSources"@en .

shapetree:AllowAll
  a :ShapeTree ;
  rdfs:comment "If no matching :contains ShapeTree is found, allow all types of unexpected content"@en ;
  rdfs:isDefinedBy <http://www.w3.org/ns/shapetree> ;
  rdfs:label "Allow All"@en .

shapetree:AllowNone
  a :ShapeTree ;
  rdfs:comment "If no matching :contains ShapeTree is found, do not allow any content"@en ;
  rdfs:isDefinedBy <http://www.w3.org/ns/shapetree> ;
  rdfs:label "Allow None"@en .

# ShapeTreeContainer IRI (maps to ldp:Container)
#############################################################################
# An IRI that represents a generalized container used in a ShapeTree
#############################################################################
shapetree:ShapeTreeContainer
  rdfs:comment "Describes a generalized container within a ShapeTree ecosystem"@en ;
  rdfs:isDefinedBy <http://www.w3.org/ns/shapetree> ;
  rdfs:label "ShapeTreeContainer"@en .


# ShapeTreeResource IRI (maps to ldp:Resource)
#############################################################################
# An IRI that represents a generalized resource used in a ShapeTree
#############################################################################
shapetree:ShapeTreeResource
  rdfs:comment "Describes a generalized RDF resource (non-container) within a ShapeTree ecosystem"@en ;
  rdfs:isDefinedBy <http://www.w3.org/ns/shapetree> ;
  rdfs:label "ShapeTreeResource"@en .

# ShapeTreeNonRDFResource IRI (maps to ldp:NonRDFSource)
#############################################################################
# An IRI that represents a generalized resource used in a ShapeTree
#############################################################################
shapetree:ShapeTreeNonRDFResource
  rdfs:comment "Describes a generalized non RDF / binary content within a ShapeTree ecosystem"@en ;
  rdfs:isDefinedBy <http://www.w3.org/ns/shapetree> ;
  rdfs:label "ShapeTreeResource"@en .


# ShapeTreeReference class
#############################################################################
# A ShapeTreeReference provides the necessary context to associate instance
# data between related ShapeTrees via a ShapePath
#############################################################################
shapetree:ShapeTreeReference
  a rdfs:Class ;
  rdfs:comment "Describes how a ShapeTree references another ShapeTree via a ShapePath"@en ;
  rdfs:isDefinedBy <http://www.w3.org/ns/shapetree> ;
  rdfs:label "ShapeTreeReference"@en .

#
# Properties in domain of ShapeTreeReference
#
shapetree:traverseViaShapePath
  a owl:DatatypeProperty ;
  rdfs:domain :ShapeTreeReference ;
  rdfs:range xsd:string ;
  rdfs:comment "Describes how one ShapeTree traverses its instance data to reach another ShapeTree"@en ;
  rdfs:isDefinedBy <http://www.w3.org/ns/shapetree> ;
  rdfs:label "Traverse Via ShapePath"@en .


#
# Properties in range of ShapeTreeDecoratorIndex
#
shapetree:hasShapeTreeDecoratorIndex
  a owl:ObjectProperty ;
  rdfs:range :ShapeTreeDecoratorIndex ;
  rdfs:isDefinedBy <http://www.w3.org/ns/shapetree> ;
  rdfs:label "Has ShapeTree Decorator Index"@en .

# ShapeTreeDecoratorIndex class
#############################################################################
# A ShapeTreeDecoratorIndex details a ShapeTree in a human-readable way.
# It is primarily used for use cases where a ShapeTree must be described to
# a user for purposes of authorization.
#############################################################################
shapetree:ShapeTreeDecoratorIndex
  a rdfs:Class ;
  rdfs:comment "Provides an index of SKOS poly-hierarchies which can be used to describe a ShapeTree"@en ;
  rdfs:isDefinedBy <http://www.w3.org/ns/shapetree> ;
  rdfs:label "ShapeTreeDecoratorIndex"@en .

# Properties in domain of ShapeTreeDecoratorIndex
#########################################################
shapetree:hasSeries
  a owl:ObjectProperty ;
  rdfs:domain :ShapeTreeDecoratorIndex ;
  rdfs:range :ShapeTreeDecoratorSeries ;
  rdfs:comment "Links between a ShapeTreeDecoratorIndex and a ShapeTreeDecoratorSeries"@en ;
  rdfs:isDefinedBy <http://www.w3.org/ns/shapetree> ;
  rdfs:label "Has Series"@en .

# ShapeTreeDecoratorSeries class
#############################################################################
# A ShapeTreeDecoratorSeries details a versioned set of ShapeTreeDecoratorHierarchy classes
# Primary use is grouping TreeDecoratorHierarchy instances by a common discriminator
# such as language or intended audience
#############################################################################
shapetree:ShapeTreeDecoratorSeries
  a rdfs:Class ;
  rdfs:comment "Groups a set of ShapeTreeDecoratorHierarchy by a given discriminator"@en ;
  rdfs:isDefinedBy <http://www.w3.org/ns/shapetree> ;
  rdfs:label "ShapeTreeDecoratorSeries"@en .

#
# Properties in domain of ShapeTreeDecoratorSeries
#
shapetree:hasHierarchy
  a owl:ObjectProperty ;
  rdfs:domain :ShapeTreeDecoratorSeries ;
  rdfs:range :ShapeTreeDecoratorHierarchy ;
  rdfs:comment "Links between a ShapeTreeDecoratorSeries and a ShapeTreeDecoratorHierarchy"@en ;
  rdfs:isDefinedBy <http://www.w3.org/ns/shapetree> ;
  rdfs:label "Has Hierarchy"@en .

# ShapeTreeDecoratorHierarchy class
#############################################################################
# A ShapeTreeDecoratorHierarchy details a versioned SKOS poly-hierarchy that describes
# a ShapeTree in a given language or format for an intended audience
# (decreased cognitivty ability, etc.)
#############################################################################
shapetree:ShapeTreeDecoratorHierarchy
  a rdfs:Class ;
  rdfs:comment "Describes a SKOS poly-hierarchy for purproses of labeling a ShapeTree"@en ;
  rdfs:isDefinedBy <http://www.w3.org/ns/shapetree> ;
  rdfs:label "ShapeTreeDecoratorHierarchy"@en .

# Properties in domain of ShapeTreeDecoratorHierarchy
#########################################################
shapetree:hasVersion
  a owl:DatatypeProperty ;
  rdfs:domain :ShapeTreeDecoratorHierarchy ;
  rdfs:range xsd:string ;
  rdfs:comment "Describes the version of a ShapeTreeDecoratorHierarchy"@en ;
  rdfs:isDefinedBy <http://www.w3.org/ns/shapetree> ;
  rdfs:label "Has Version"@en .

shapetree:hasSHA256Hash
  a owl:DatatypeProperty ;
  rdfs:domain :ShapeTreeDecoratorHierarchy ;
  rdfs:range xsd:string ;
  rdfs:comment "Describes the SHA-256 of a ShapeTreeDecoratorHierarchy"@en ;
  rdfs:isDefinedBy <http://www.w3.org/ns/shapetree> ;
  rdfs:label "Has SHA-256 Hash"@en .

shapetree:hasSkosGraph
  a owl:ObjectProperty ;
  rdfs:domain :ShapeTreeDecoratorHierarchy ;
  rdfs:range :ShapeTreeLabel ;
  rdfs:comment "Represents the IRI to the SKOS graph described by ShapeTreeDecoratorHierarchy instance"@en ;
  rdfs:isDefinedBy <http://www.w3.org/ns/shapetree> ;
  rdfs:label "Has SKOS Graph"@en .

# ShapeTreeLabel class
#############################################################################
# A ShapeTreeLabel details the association between a label within a SKOS graph
# (detailed by ShapeTreeDecoratorHierarchy) and a ShapeTree
#############################################################################
shapetree:ShapeTreeLabel
  a rdfs:Class ;
  rdfs:comment "Describes the association between a SKOS label and a ShapeTree"@en ;
  rdfs:isDefinedBy <http://www.w3.org/ns/shapetree> ;
  rdfs:label "ShapeTreeLabel"@en .


# Properties in the range of ShapeTreeLocator
#########################################################
shapetree:hasShapeTreeLocator
  a owl:ObjectProperty ;
  rdfs:range :ShapeTreeLocator ;
  rdfs:comment "Represents the association between a subject an one or more ShapeTreeLocator"@en ;
  rdfs:isDefinedBy <http://www.w3.org/ns/shapetree> ;
  rdfs:label "Has ShapeTree Locator"@en .


# ShapeTreeLocator class
#############################################################################
# A ShapeTreeLocator describes a planted ShapeTree in a container with enough
# information to traverse from the current container to the root
#############################################################################
shapetree:ShapeTreeLocator
  a rdfs:Class ;
  rdfs:comment "Describes a planted ShapeTree in a container with enough information to traverse from the current container to the root"@en ;
  rdfs:isDefinedBy <http://www.w3.org/ns/shapetree> ;
  rdfs:label "ShapeTreeLocator"@en .

# Properties in domain of ShapeTreeLocator
#########################################################

shapetree:hasShapeTreeInstanceRoot
  a owl:ObjectProperty ;
  rdfs:domain :ShapeTreeLocator ;
  rdfs:comment "Represents the IRI of a root of a planted ShapeTree hierarchy"@en ;
  rdfs:isDefinedBy <http://www.w3.org/ns/shapetree> ;
  rdfs:label "Has ShapeTree Instance Root"@en .

shapetree:hasRootShapeTree
  a owl:ObjectProperty ;
  rdfs:domain :ShapeTreeLocator ;
  rdfs:range :ShapeTree ;
  rdfs:comment "Represents the ShapeTree that is planted at the root of the ShapeTree hierarchy.  For flat structures, hasRootShapeTree and hasShapeTree will be the same."@en ;
  rdfs:isDefinedBy <http://www.w3.org/ns/shapetree> ;
  rdfs:label "Has Root ShapeTree"@en .


################################################################
# A generalized predicate for linking a class to a ShapeTree
################################################################
shapetree:hasShapeTree
  a owl:ObjectProperty ;
  rdfs:range :ShapeTree ;
  rdfs:comment "Represents the IRI of a ShapeTree that is referenced by some subject"@en ;
  rdfs:isDefinedBy <http://www.w3.org/ns/shapetree> ;
  rdfs:label "Has ShapeTree Instance Root"@en .
