# See details within this document for linkage to specification and purpose.
# This ontology file is a non-normative supporting document.

# Solid terms ontology

## Ontology preferred namespace prefix and URI
prefix solid: <http://www.w3.org/ns/solid/terms#>

## Other namespaces used
### Core W3C ontologies (OWL 2 reserved vocabulary)
prefix rdf: <http://www.w3.org/1999/02/22-rdf-syntax-ns#>
prefix rdfs: <http://www.w3.org/2000/01/rdf-schema#>
prefix owl: <http://www.w3.org/2002/07/owl#>
prefix xsd: <http://www.w3.org/2001/XMLSchema#>
### Other ontologies
prefix dc: <http://purl.org/dc/terms/>
prefix ldp: <http://www.w3.org/ns/ldp#>
prefix log: <http://www.w3.org/2000/10/swap/log#>
prefix vann: <http://purl.org/vocab/vann/>


## Ontology
<http://www.w3.org/ns/solid/terms>
    a owl:Ontology ;
    rdfs:label "Solid Terms ontology"@en ;
    rdfs:comment "Solid, derived from social linked data, is a proposed set of conventions and tools for building decentralized social applications based on Linked Data principles."@en ;
    rdfs:isDefinedBy <http://www.w3.org/ns/solid/terms> ;
    rdfs:seeAlso
        <https://solid.github.io/specification/> ;
    dc:issued "2015-11-16"^^xsd:date ;
    dc:modified "2015-12-18"^^xsd:date ;
    dc:modified "2015-12-20"^^xsd:date ;
    dc:modified "2016-01-04"^^xsd:date ;
    dc:modified "2016-02-05"^^xsd:date ;
    dc:modified "2016-03-11"^^xsd:date ;
    dc:modified "2016-05-17"^^xsd:date ;
    dc:modified "2017-08-15"^^xsd:date ;
    dc:modified "2017-08-16"^^xsd:date ;
    dc:modified "2017-08-17"^^xsd:date ;
    dc:modified "2018-01-24"^^xsd:date ;
    dc:modified "2018-10-24"^^xsd:date ;
    dc:modified "2018-10-25"^^xsd:date ;
    dc:modified "2018-10-26"^^xsd:date ;
    dc:modified "2018-11-07"^^xsd:date ;
    dc:modified "2019-01-22"^^xsd:date ;
    dc:modified "2020-12-18"^^xsd:date ;
    vann:preferredNamespacePrefix "solid" ;
    vann:preferredNamespaceUri "http://www.w3.org/ns/solid/terms#"^^xsd:anyURI .

### Classes
solid:Account
    a rdfs:Class ;
    dc:issued "2016-05-17"^^xsd:date ;
    rdfs:comment "A Solid account."@en ;
    rdfs:isDefinedBy <http://www.w3.org/ns/solid/terms> ;
    rdfs:label "Account"@en .

solid:Inbox
    a rdfs:Class ;
    dc:issued "2015-11-16"^^xsd:date ;
    dc:modified "2018-10-24"^^xsd:date ;
    rdfs:comment "A resource containing notifications."@en ;
    rdfs:isDefinedBy <http://www.w3.org/ns/solid/terms> ;
    rdfs:label "Inbox"@en .

solid:ListedDocument
    a rdfs:Class ;
    dc:issued "2015-11-16"^^xsd:date ;
    dc:modified "2018-01-24"^^xsd:date ;
    rdfs:comment "Listed Type Index is a registry of resources that are publicly discoverable by outside users and applications."@en ;
    rdfs:isDefinedBy <http://www.w3.org/ns/solid/terms> ;
    rdfs:label "Listed Type Index"@en .

solid:Notification
    a rdfs:Class ;
    dc:issued "2015-12-18"^^xsd:date ;
    dc:modified "2015-12-20"^^xsd:date ;
    dc:modified "2018-10-25"^^xsd:date ;
    rdfs:comment "A notification resource."@en ;
    rdfs:isDefinedBy <http://www.w3.org/ns/solid/terms> ;
    rdfs:label "Notification"@en .

solid:Patch
    a rdfs:Class ;
    dc:issued "2017-08-17"^^xsd:date ;
    rdfs:comment "A patch expresses conditional modifications to a resource that has an RDF-based representation."@en ;
    rdfs:isDefinedBy <http://www.w3.org/ns/solid/terms> ;
    rdfs:label "Patch"@en .

solid:Timeline
    a rdfs:Class ;
    dc:issued "2016-01-04"^^xsd:date ;
    rdfs:comment "A resource containing time ordered items and sub-containers.  Sub-containers may be desirable in file based systems to split the timeline into logical components e.g. /yyyy-mm-dd/ as used in ISO 8061."@en ;
    rdfs:isDefinedBy <http://www.w3.org/ns/solid/terms> ;
    rdfs:label "Timeline"@en .

solid:TypeIndex
    a rdfs:Class ;
    dc:issued "2016-02-05"^^xsd:date ;
    rdfs:comment "A index of type registries for resources. Applications can register the RDF type they use and list them in the index resource."@en ;
    rdfs:isDefinedBy <http://www.w3.org/ns/solid/terms> ;
    rdfs:label "Type index"@en .

solid:TypeRegistration
    a rdfs:Class ;
    dc:issued "2018-01-24"^^xsd:date ;
    rdfs:comment "The registered types that map a RDF classes/types to their locations using either `instance` or `instanceContainer` property."@en ;
    rdfs:isDefinedBy <http://www.w3.org/ns/solid/terms> ;
    rdfs:label "Type Registration"@en .

solid:UnlistedDocument
    a rdfs:Class ;
    dc:issued "2018-01-24"^^xsd:date ;
    rdfs:comment "Unlisted Type Index is a registry of resources that are private to the user and their apps, for types that are not publicly discoverable."@en ;
    rdfs:isDefinedBy <http://www.w3.org/ns/solid/terms> ;
    rdfs:label "Unlisted Type Index"@en .

### Properties
solid:account
    a rdf:Property ;
    dc:issued "2016-05-17"^^xsd:date ;
    dc:modified "2018-01-24"^^xsd:date ;
    rdfs:comment "A solid account belonging to an Agent."@en ;
    rdfs:isDefinedBy <http://www.w3.org/ns/solid/terms> ;
    rdfs:label "account"@en .

solid:deletes
    a rdf:Property, owl:ObjectProperty, owl:FunctionalProperty ;
    dc:issued "2017-08-17"^^xsd:date ;
    rdfs:comment "The triple patterns this patch removes from the document."@en ;
    rdfs:isDefinedBy <http://www.w3.org/ns/solid/terms> ;
    rdfs:label "deletes"@en ;
    rdfs:domain solid:Patch ;
    rdfs:range log:Formula .

solid:forClass
    a rdf:Property ;
    dc:issued "2018-01-24"^^xsd:date ;
    rdfs:comment "A class that is used to map an listed or unlisted type index."@en ;
    rdfs:isDefinedBy <http://www.w3.org/ns/solid/terms> ;
    rdfs:label "registry class"@en .

solid:identityProvider
    owl:deprecated true ;
    a rdf:Property ;
    dc:issued "2020-12-18"^^xsd:date ;
    rdfs:comment "An identity provider that can be used to assert ownership of a WebID."@en ;
    rdfs:isDefinedBy <http://www.w3.org/ns/solid/terms> ;
    rdfs:label "identity provider"@en .

solid:inbox
    owl:deprecated true ;
    a rdf:Property ;
    dc:issued "2015-11-16"^^xsd:date ;
    dc:modified "2016-02-05"^^xsd:date ;
    dc:modified "2018-10-25"^^xsd:date ;
    owl:equivalentProperty ldp:inbox ;
    rdfs:subPropertyOf ldp:inbox ;
    rdfs:comment "Deprecated pointer to a Linked Data Notifications inbox; please use http://www.w3.org/ns/ldp#inbox instead."@en ;
    rdfs:isDefinedBy <http://www.w3.org/ns/solid/terms> ;
    rdfs:label "inbox (deprecated)"@en .

solid:inserts
    a rdf:Property, owl:ObjectProperty, owl:FunctionalProperty ;
    dc:issued "2017-08-17"^^xsd:date ;
    rdfs:comment "The triple patterns this patch adds to the document."@en ;
    rdfs:isDefinedBy <http://www.w3.org/ns/solid/terms> ;
    rdfs:label "inserts"@en ;
    rdfs:domain solid:Patch ;
    rdfs:range log:Formula .

solid:instance
    a rdf:Property ;
    dc:issued "2018-01-24"^^xsd:date ;
    rdfs:comment "Maps a type to an individual resource, typically an index or a directory listing resource."@en ;
    rdfs:isDefinedBy <http://www.w3.org/ns/solid/terms> ;
    rdfs:label "instance"@en .

solid:instanceContainer
    a rdf:Property ;
    dc:issued "2018-01-24"^^xsd:date ;
    rdfs:comment "Maps a type to a container which the client would have to list to get the instances of that type."@en ;
    rdfs:isDefinedBy <http://www.w3.org/ns/solid/terms> ;
    rdfs:label "instance container"@en .

solid:loginEndpoint
    a rdf:Property ;
    dc:issued "2015-11-16"^^xsd:date ;
    rdfs:comment "The login URI of a given server."@en ;
    rdfs:isDefinedBy <http://www.w3.org/ns/solid/terms> ;
    rdfs:label "loginEndpoint"@en .

solid:logoutEndpoint
    a rdf:Property ;
    dc:issued "2015-11-16"^^xsd:date ;
    rdfs:comment "The logout URI of a given server."@en ;
    rdfs:isDefinedBy <http://www.w3.org/ns/solid/terms> ;
    rdfs:label "logoutEndpoint"@en .

solid:notification
    a rdf:Property ;
    dc:issued "2016-03-11"^^xsd:date ;
    dc:modified "2018-10-25"^^xsd:date ;
    rdfs:comment "Notification resource for an inbox."@en ;
    rdfs:isDefinedBy <http://www.w3.org/ns/solid/terms> ;
    rdfs:label "notification"@en .

solid:oidcIssuer
    owl:deprecated true ;
    owl:equivalentProperty solid:identityProvider ;
    a rdf:Property ;
    dc:issued "2017-08-15"^^xsd:date ;
    dc:modified "2017-08-16"^^xsd:date ;
    dc:modified "2020-12-18"^^xsd:date ;
    rdfs:comment "The preferred OpenID Connect issuer URI for a given Web ID."@en ;
    rdfs:isDefinedBy <http://www.w3.org/ns/solid/terms> ;
    rdfs:label "oidc issuer"@en ;
    rdfs:subPropertyOf <http://openid.net/specs/connect/1.0/issuer> .

solid:patches
    a rdf:Property, owl:ObjectProperty ;
    dc:issued "2017-08-17"^^xsd:date ;
    rdfs:comment "The document to which this patch applies."@en ;
    rdfs:isDefinedBy <http://www.w3.org/ns/solid/terms> ;
    rdfs:label "patches"@en ;
    rdfs:domain solid:Patch ;
    rdfs:range rdfs:Resource .

solid:privateTypeIndex
    a rdf:Property ;
    dc:issued "2018-01-24"^^xsd:date ;
    rdfs:comment "Points to an unlisted type index resource."@en ;
    rdfs:range <#UnlistedDocument> ;
    rdfs:isDefinedBy <http://www.w3.org/ns/solid/terms> ;
    rdfs:label "private type index"@en .

solid:publicTypeIndex
    a rdf:Property ;
    dc:issued "2018-01-24"^^xsd:date ;
    rdfs:subPropertyOf solid:typeIndex ;
    rdfs:comment "Points to a listed type index resource."@en ;
    rdfs:range <#ListedDocument> ;
    rdfs:isDefinedBy <http://www.w3.org/ns/solid/terms> ;
    rdfs:label "public type index"@en .

solid:read
    a rdf:Property ;
    dc:issued "2015-12-18"^^xsd:date ;
    rdfs:comment "Indicates if a message has been read or not. This property should have a boolean datatype."@en ;
    rdfs:isDefinedBy <http://www.w3.org/ns/solid/terms> ;
    rdfs:domain <http://rdfs.org/sioc/ns#Post> ;
    rdfs:label "read"@en .

solid:storageQuota
    a rdf:Property, owl:DatatypeProperty ;
    dc:issued "2018-10-26"^^xsd:date ;
    dc:modified "2018-11-07"^^xsd:date ;
    dc:modified "2019-01-22"^^xsd:date ;
    rdfs:comment "The quota of non-volatile memory that is available for the account (in bytes)"@en ;
    rdfs:isDefinedBy <http://www.w3.org/ns/solid/terms> ;
    rdfs:domain solid:Account ;
    rdfs:label "Non-volatile memory quota"@en .

solid:storageUsage
    a rdf:Property, owl:DatatypeProperty ;
    dc:issued "2019-01-22"^^xsd:date ;
    rdfs:comment "The amount of non-volatile memory that the account have used (in bytes)"@en ;
    rdfs:isDefinedBy <http://www.w3.org/ns/solid/terms> ;
    rdfs:domain solid:Account ;
    rdfs:label "Non-volatile memory usage"@en .

solid:typeIndex
    a rdf:Property ;
    dc:issued "2016-02-05"^^xsd:date ;
    rdfs:comment "Points to a TypeIndex resource."@en ;
    rdfs:range <#TypeIndex> ;
    rdfs:isDefinedBy <http://www.w3.org/ns/solid/terms> ;
    rdfs:label "type index"@en .

solid:timeline
    a rdf:Property ;
    dc:issued "2016-01-04"^^xsd:date ;
    rdfs:comment "Timeline for a given resource."@en ;
    rdfs:isDefinedBy <http://www.w3.org/ns/solid/terms> ;
    rdfs:label "timeline"@en .

solid:where
    a rdf:Property, owl:ObjectProperty, owl:FunctionalProperty ;
    dc:issued "2017-08-17"^^xsd:date ;
    rdfs:comment "The conditions the document and the inserted and deleted triple patterns need to satisfy in order for the patch to be applied."@en ;
    rdfs:isDefinedBy <http://www.w3.org/ns/solid/terms> ;
    rdfs:label "where"@en ;
    rdfs:domain solid:Patch ;
    rdfs:range log:Formula .
