# Ontology preferred namespace prefix and URI
@prefix ws: <http://www.w3.org/ns/pim/space#> .
# Related Ontology
@prefix doc: <http://www.w3.org/2000/10/swap/pim/doc#> .

@prefix rdfs: <http://www.w3.org/2000/01/rdf-schema#> .
@prefix owl: <http://www.w3.org/2002/07/owl#> .
@prefix dc: <http://purl.org/dc/elements/1.1/> .
@prefix foaf: <http://xmlns.com/foaf/0.1/> .
@prefix gen: <http://www.w3.org/2006/gen/ont#> .
@prefix rdf: <http://www.w3.org/1999/02/22-rdf-syntax-ns#> .
@prefix ui: <http://www.w3.org/ns/ui#> .

<http://www.w3.org/ns/pim/space>
    dc:title "Workspace Ontology" ;
    rdfs:comment """This ontology is for use in describing
Workspaces.  Workspaces are place where data is stored and asscoiated prolices of privacy.
A given application typically stores information in several different
workspaces, some being user private, some shared, and some public.
it is crucial that the user has easy control over the destiny of information.

Goals then are that the user can:
      - create workspaces
      - easily understand which workspace data is going into
      - understand what the implications of that are
      - (later) set ACLS on them
      - publish apropriate use policies for them""" ;
    doc:version "$Id: space.ttl,v 1.2 2015/06/24 18:42:14 asambra Exp $" .

ws:ConfigurationFile
    rdfs:subClassOf gen:InformationResource .

ws:ControlledStorage
    a :Class;
    rdfs:comment """A storage is a space of URIs in which you can individually control for each resource
who has access to it.""" ;
    rdfs:label "access controlled storage" ;
    rdfs:subClassOf ws:Storage .

ws:masterWorkspace
    rdfs:comment """This is a workspace for storing the
information about the other workspaces.
As a user, you normally don't have to worry about it.""" ;
    rdfs:label "Master Workspace"@en ;
    rdfs:subClassOf ws:PrivateWorkspace .

ws:PersonalStorage
    a :Class;
    rdfs:comment """A personal storage is a space of URIs in which you and only you have access to data,
you cannot give access to anyone else.""" ;
    rdfs:label "personal storage" ;
    rdfs:subClassOf ws:Storage .

ws:PrivateWorkspace
    rdfs:comment "Access only by the you, the user." ;
    rdfs:label "Private workspace";
    rdfs:subClassOf ws:Workspace .

ws:PublicStorage
    a :Class;
    rdfs:comment """A public storage is a space of URIs in which you have access to data,
and all data is accessible to anyone without control.""";
    rdfs:label "public storage";
    rdfs:subClassOf ws:Storage .

ws:PublicWorkspace
    rdfs:comment """Aceess is open to the public. Anything in a public workspace
can be accesed by anyone.""";
    rdfs:label "Public workspace";
    rdfs:subClassOf ws:Workspace .

ws:PreferencesWorkspace
    rdfs:comment """AAceess may not be open to the public.
Contains preferences resources""" ;
    rdfs:label "Preferences workspace" ;
    rdfs:subClassOf ws:Workspace .

ws:SharedWorkspace
    rdfs:comment "Access is to some but not all people." ;
    rdfs:label "Shared workspace" ;
    rdfs:subClassOf ws:Workspace .

ws:Storage
    a rdfs:Class;
    rdfs:comment "A storage is a space of URIs in which you have access to data.";
    rdfs:label "storage" .

ws:Workspace
    a rdfs:Class;
    rdfs:comment """Workspaces are place where data is stored, and associated polices of privacy.
A given application typically stores information in several different
workspaces, some being user private, some shared, and some public.
""";
    rdfs:label "workspace";
    owl:disjointUnionOf  (
        ws:PrivateWorkspace
        ws:SharedWorkspace
        ws:PublicWorkspace ) .

ws:masterWorkspace
    a rdf:Property ;
    rdfs:domain foaf:Agent ;
    rdfs:label "master workspace"@en ;
    rdfs:range ws:MasterWorkspace .

ws:preferencesFile
    a rdf:Property ;
    rdfs:domain foaf:Agent ;
    rdfs:label "preferences file" ;
    rdfs:range ws:ConfigurationFile .

ws:storage
    a rdf:Property;
    rdfs:comment "The storage in which this workspace is";
    rdfs:label "storage" ;
    rdfs:range ws:Storage ;
    owl:inverse [ :label "workspace included" ] .

ws:uriPrefix
    a rdf:Property, owl:DatatypeProperty ;
    rdfs:comment """URIs which start with this string are in this workspace or storage.
This may be used for constructing URIs for new storage resources.
""";
    rdfs:label "URI prefix" ;
    ui:prompt "Give the first part of the URis in this workspace" .

ws:workspace
    a rdf:Property ;
    rdfs:label "workspace"@en ;
    rdfs:range ws:Workspace .
