# See details within this document for linkage to specification and purpose.
# This ontology file is a non-normative supporting document.

# Vocabulary Annotation ontology

## Ontology preferred namespace prefix and URI
prefix vann: <http://purl.org/vocab/vann/>

## Other namespaces used
### Core W3C ontologies (OWL 2 reserved vocabulary)
prefix rdf: <http://www.w3.org/1999/02/22-rdf-syntax-ns#>
prefix rdfs: <http://www.w3.org/2000/01/rdf-schema#>
prefix owl: <http://www.w3.org/2002/07/owl#>
prefix xsd: <http://www.w3.org/2001/XMLSchema#>
### Other ontologies
prefix dcterms: <http://purl.org/dc/terms/>
prefix foaf: <http://xmlns.com/foaf/0.1/>

## Ontology
<http://purl.org/vocab/vann/>
    a owl:Ontology ;
    rdfs:label "Vocabulary annotation ontology"@en ;
    rdfs:comment "The vocabulary annotation ontology is used to describe an ontology and the terms it defines."@en ;
    rdfs:isDefinedBy <http://purl.org/vocab/vann/> ;
    rdfs:seeAlso <https://vocab.org/vann/> ;
    vann:preferredNamespacePrefix "vann" ;
    vann:preferredNamespaceUri "http://purl.org/vocab/vann/"^^xsd:anyURI ;
    dcterms:creator [
        rdfs:seeAlso <http://iandavis.com/id/me> ;
        foaf:name "Ian Davis" ;
        ] ;
    dcterms:issued "2005-04-01"^^xsd:date ;
    owl:priorVersion <http://purl.org/vocab/vann/vann-vocab-20040305> .

## Property
vann:changes
    a rdf:Property ;
    rdfs:subPropertyOf rdfs:seeAlso ;
    rdfs:label "changes" ;
    rdfs:comment "A reference to a resource that describes changes between this version of a vocabulary and the previous." ;
    rdfs:isDefinedBy <http://purl.org/vocab/vann/> .

vann:example
    a rdf:Property ;
    rdfs:subPropertyOf rdfs:seeAlso ;
    rdfs:label "Example"@en ;
    rdfs:comment "A reference to a resource that provides an example of how this resource can be used."@en ;
    rdfs:isDefinedBy <http://purl.org/vocab/vann/> .

vann:preferredNamespacePrefix
    a rdf:Property ;
    rdfs:label "Preferred namespace prefix"@en ;
    rdfs:comment "The preferred namespace prefix to use when serialising terms from this vocabulary to a compact URI (CURIE)."@en ;
    rdfs:isDefinedBy <http://purl.org/vocab/vann/> .

vann:preferredNamespaceUri
    a rdf:Property ;
    rdfs:label "Preferred namespace URI"@en ;
    rdfs:comment "The preferred namespace URI to use when substituting the prefix in a compact URI."@en ;
    rdfs:isDefinedBy <http://purl.org/vocab/vann/> .

vann:termGroup
    a rdf:Property ;
    rdfs:label "Term group"@en ;
    rdfs:comment "A group of related terms in a vocabulary."@en ;
    rdfs:isDefinedBy <http://purl.org/vocab/vann/> .

vann:usageNote
    a rdf:Property ;
    rdfs:subPropertyOf rdfs:seeAlso ;
    rdfs:label "Usage note"@en ;
    rdfs:comment "A reference to a resource that provides information on how this resource is meant to be used."@en ;
    rdfs:isDefinedBy <http://purl.org/vocab/vann/> .
